RPC going through with keys paired with property (still one assume)

doc/tutorial/code/solutions/Ex12.MAC.fst
@@ -22,6 +22,7 @@ open STx
 open MRefx
 
 module SHA1 = Ex12.SHA1
+module SEM = FStar.StrongExcludedMiddle
 (* open FStar.List.Tot *)
 
 (* (\* key log *\) *)
@@ -42,6 +43,9 @@ module SHA1 = Ex12.SHA1
 
 (* type pkey (p:string -> GTot bool) = k:key{token key_log (associated_to k p)} *)
 
+let pred_to_dec_ghost (#a:Type) (p:a -> Tot Type0 (* prop *))
+  : a -> GTot bool
+= fun x -> SEM.strong_excluded_middle (p x)
 
 (* ---- specification *)
 
@@ -49,14 +53,15 @@ module SHA1 = Ex12.SHA1
 (* We make the MAC.key abstract so that it cannot be accessed by
    the adversary *)
 
-abstract type key=SHA1.key
+abstract type key= SHA1.key * (text -> GTot bool)
+assume private val key_unicity (k1 k2 : key) : Lemma (requires (fst k1 == fst k2)) (ensures (snd k1 == snd k2))
 
 (* we attach an authenticated properties to each key,
    used as a pre-condition for MACing and
    a postcondition of MAC verification *)
 
-assume type key_prop : key -> text -> Type0
-type pkey (p:(text -> Type)) = k:key{key_prop k == p}
+let key_prop : key -> text -> Type0 = fun k t -> snd k t
+type pkey (p:(text -> Type)) = k:key{forall x. key_prop k x <==> p x}
 
 (* to model authentication, we log all genuine calls
    to MACs; the ideal implementation below uses the
@@ -64,13 +69,14 @@ type pkey (p:(text -> Type)) = k:key{key_prop k == p}
 
 type tag = SHA1.tag
 
+noeq
 type entry =
   | Entry : k:key
          -> t:text{key_prop k t}
          -> m:tag
          -> entry
 
-(* the log needs to be private so the adversary cannot 
+(* the log needs to be private so the adversary cannot
    add or remove entries *)
 
 (* let key_prop k t =  exists p. token key_log (associated_to k p) /\ p t *)
@@ -79,37 +85,41 @@ private type log_t = ref (list entry)
 let log:log_t = STx.alloc _ []
 
 // BEGIN: MacSpec
-val keygen: p:(text -> Type) -> St (pkey p)
-val mac:    k:key -> t:text{key_prop k t} -> ST tag 
-  (requires (fun h -> True)) 
+val keygen: p:(text -> Type0) -> St (pkey p)
+val mac:    k:key -> t:text{key_prop k t} -> ST tag
+  (requires (fun h -> True))
   (ensures (fun h x h' -> modifies (Set.singleton (addr_of log)) h h'))
-val verify: k:key -> t:text -> tag -> ST (b:bool{b ==> key_prop k t}) 
-  (requires (fun h -> True)) 
+val verify: k:key -> t:text -> tag -> ST (b:bool{b ==> key_prop k t})
+  (requires (fun h -> True))
   (ensures (fun h x h' -> modifies Set.empty h h'))
 // END: MacSpec
 
 (* ---- implementation *)
 
 let keygen (p: (text -> Type)) =
-  let k:key = sample keysize in
-  assume (key_prop k == p);
+  let k:key = sample keysize, pred_to_dec_ghost p in
+  assert (forall x. key_prop k x <==> p x);
   k
 
 
 let mac k t =
-  let m = hmac_sha1 k t in
+  let m = hmac_sha1 (fst k) t in
   log := Entry k t m :: !log;
   m
 
 let verify k text tag =
   (* to verify, we simply recompute & compare *)
-  let m= hmac_sha1 k text in
+  let m = hmac_sha1 (fst k) text in
   let verified = (Platform.Bytes.equalBytes m tag) in
-  let found =
-    Some?
-      (List.Tot.find
-        (fun (Entry k' text' tag') -> Platform.Bytes.equalBytes k k' && Platform.Bytes.equalBytes text text')
-        !log) in
+  let equal_entry (Entry k' text' tag') =
+    Platform.Bytes.equalBytes (fst k) (fst k') && Platform.Bytes.equalBytes text text'
+  in
+  let entry_opt = List.Tot.find equal_entry !log in
+  let found = Some? entry_opt in
+  begin match entry_opt with
+    | None -> ()
+    | Some (Entry k' _ _) -> key_unicity k k'
+  end ;
 
   (* plain, concrete implementation (ignoring the log) *)
 //verified
